pulse/lib/steel/pulse/Pulse.Checker.Auto.Util.fst
@@ -1,0 +1,55 @@
+module Pulse.Checker.Auto.Util
+open Pulse.Syntax
+open Pulse.Typing
+open Pulse.Checker.Common
+open Pulse.Checker.Framing
+open Pulse.Checker.VPropEquiv
+module Metatheory = Pulse.Typing.Metatheory
+module T = FStar.Tactics
+
+let k_elab_unit (g:env) (ctxt:term)
+  : continuation_elaborator g ctxt g ctxt
+  = fun p r -> r
+
+let k_elab_trans (#g0 #g1 #g2:env) (#ctxt0 #ctxt1 #ctxt2:term)
+                 (k0:continuation_elaborator g0 ctxt0 g1 ctxt1)
+                 (k1:continuation_elaborator g1 ctxt1 g2 ctxt2 { g1 `env_extends` g0})
+   : continuation_elaborator g0 ctxt0 g2 ctxt2
+   = fun post_hint res -> k0 post_hint (k1 post_hint res)
+
+let k_elab_equiv (#g1 #g2:env) (#ctxt1 #ctxt1' #ctxt2 #ctxt2':term)                 
+                 (k:continuation_elaborator g1 ctxt1 g2 ctxt2)
+                 (d1:vprop_equiv g1 ctxt1 ctxt1')
+                 (d2:vprop_equiv g2 ctxt2 ctxt2')
+  : continuation_elaborator g1 ctxt1' g2 ctxt2'
+  =  fun post_hint res -> 
+        let framing_token2 : frame_for_req_in_ctxt g2 ctxt2 ctxt2' = 
+            let d : vprop_equiv g2 (Tm_Star ctxt2' Tm_Emp) ctxt2 = 
+              VE_Trans _ _ _ _ (VE_Comm _ _ _) (VE_Trans _ _ _ _ (VE_Unit _ _) (VE_Sym _ _ _ d2)) in
+            (| Tm_Emp, emp_typing, d |)
+        in
+        let framing_token1 : frame_for_req_in_ctxt g1 ctxt1' ctxt1 = 
+            let d = VE_Trans _ _ _ _ (VE_Comm _ _ _) (VE_Trans _ _ _ _ (VE_Unit _ _) d1) in
+            (| Tm_Emp, emp_typing, d |)
+        in
+        let (| st, c, st_d |) = res in
+        if not (stateful_comp c)
+        then T.fail "Unexpected non-stateful comp in continuation elaborate"
+        else (
+            let (| _, pre_typing, _, _ |) =
+                Metatheory.(st_comp_typing_inversion (comp_typing_inversion (st_typing_correctness st_d))) in
+            let (| c', st_d' |) = Pulse.Checker.Framing.apply_frame (vprop_equiv_typing_bk pre_typing d2) st_d framing_token2 in
+            let (| st, c, st_d |) = k post_hint (| st, c', st_d' |) in
+            if not (stateful_comp c)
+            then T.fail "Unexpected non-stateful comp in continuation elaborate"
+            else 
+                let (| _, pre_typing, _, _ |) =
+                    Metatheory.(st_comp_typing_inversion (comp_typing_inversion (st_typing_correctness st_d))) in
+                let (| c', st_d' |) =
+                    Pulse.Checker.Framing.apply_frame
+                        (vprop_equiv_typing_fwd pre_typing d1)
+                        st_d
+                        framing_token1 in
+                (| st, c', st_d' |)
+        )
+
