pulse/lib/steel/pulse/Pulse.Checker.Auto.Util.fsti
@@ -1,0 +1,18 @@
+module Pulse.Checker.Auto.Util
+open Pulse.Syntax
+open Pulse.Typing
+open Pulse.Checker.Common
+
+val k_elab_unit (g:env) (ctxt:term)
+  : continuation_elaborator g ctxt g ctxt
+
+val k_elab_trans (#g0 #g1 #g2:env) (#ctxt0 #ctxt1 #ctxt2:term)
+                 (k0:continuation_elaborator g0 ctxt0 g1 ctxt1)
+                 (k1:continuation_elaborator g1 ctxt1 g2 ctxt2 { g1 `env_extends` g0})
+   : continuation_elaborator g0 ctxt0 g2 ctxt2
+
+val k_elab_equiv (#g1 #g2:env) (#ctxt1 #ctxt1' #ctxt2 #ctxt2':term)                 
+                 (k:continuation_elaborator g1 ctxt1 g2 ctxt2)
+                 (d1:vprop_equiv g1 ctxt1 ctxt1')
+                 (d2:vprop_equiv g2 ctxt2 ctxt2')
+  : continuation_elaborator g1 ctxt1' g2 ctxt2'
