pulse/lib/steel/pulse/Pulse.Checker.Common.fsti
@@ -144,4 +144,3 @@ type check_t =
   pre_typing:tot_typing g pre Tm_VProp ->
   post_hint:post_hint_opt g ->
   T.Tac (checker_result_t g pre post_hint)
-
